coq-verification/src/Concrete/PageTablesWf.v
@@ -1,0 +1,118 @@
+(*
+ * Copyright 2019 Jade Philipoom
+ *
+ * Licensed under the Apache License, Version 2.0 (the "License");
+ * you may not use this file except in compliance with the License.
+ * You may obtain a copy of the License at
+ *
+ *     https://www.apache.org/licenses/LICENSE-2.0
+ *
+ * Unless required by applicable law or agreed to in writing, software
+ * distributed under the License is distributed on an "AS IS" BASIS,
+ * WITHOUT WARRANTIES OR CONDITIONS OF ANY KIND, either express or implied.
+ * See the License for the specific language governing permissions and
+ * limitations under the License.
+ *)
+
+Require Import Coq.Lists.List.
+Require Import Coq.Arith.PeanoNat.
+Require Import Hafnium.Concrete.Datatypes.
+Require Import Hafnium.Util.Tactics.
+Require Import Hafnium.Concrete.Assumptions.Addr.
+Require Import Hafnium.Concrete.Assumptions.ArchMM.
+Require Import Hafnium.Concrete.Assumptions.Constants.
+Require Import Hafnium.Concrete.Assumptions.Datatypes.
+Require Import Hafnium.Concrete.Assumptions.PageTables.
+Require Import Hafnium.Concrete.MM.Datatypes.
+
+(* states that a table has the right number of entries at every level and doesn't
+   exceed the maximum number of levels *)
+(* TODO : could add max_block_level to this, and get the proof that tables don't
+   have blocks above level 2 *)
+Inductive page_table_wf (deref : ptable_pointer -> mm_page_table) (s : Stage)
+  : mm_page_table -> nat -> Prop :=
+| page_table_wf_last_level :
+    (* no table entries at next level down *)
+    forall (entries : list pte_t) (level : nat),
+      length entries = MM_PTE_PER_PAGE ->
+      level < max_level s ->
+      Forall (fun pte => arch_mm_pte_is_table pte level = false) entries ->
+      page_table_wf deref s {| entries := entries |} level
+| page_table_wf_step :
+    (* well-formed if the level below is also *)
+    forall (entries : list pte_t) (level : nat),
+      length entries = MM_PTE_PER_PAGE ->
+      level <= max_level s ->
+      Forall (fun pte =>
+                arch_mm_pte_is_table pte (S level) = true ->
+                let next_ptr := ptable_pointer_from_address
+                                  (arch_mm_table_from_pte pte (S level)) in
+                let next_table := deref next_ptr in
+                page_table_wf deref s next_table level) entries ->
+      page_table_wf deref s {| entries := entries |} (S level)
+.
+ 
+Definition root_ptable_wf deref (s : Stage) (root_ptable : mm_ptable) : Prop :=
+  let root_tables := ptr_from_va (va_from_pa (root root_ptable)) in
+  (length root_tables = root_table_count s
+   /\ Forall
+        (fun ptr => page_table_wf deref s (deref ptr) (max_level s))
+        root_tables).
+
+Definition address_wf (a : uintpaddr_t) (s : Stage) : Prop :=
+  (forall level, level <= max_level s -> get_index s level a < MM_PTE_PER_PAGE)
+  /\ (get_index s (max_level s + 1) a < root_table_count s).
+
+Lemma page_lookup'_ok deref s a :
+  forall level t,
+    address_wf a s ->
+    page_table_wf deref s t (pred level) ->
+    0 < level <= max_level s + 1->
+    page_lookup' deref a t level s <> None.
+Proof.
+  induction level; [|destruct (Nat.eq_dec level 0)]; basics;
+    match goal with
+    | H : address_wf _ _ |- _ => pose proof H; cbv [address_wf] in H
+    end;
+    repeat match goal with
+           | _ => progress basics
+           | _ => progress cbn [page_lookup']; cbv [get_entry]
+           | _ => progress cbn [Datatypes.entries] in *
+           | _ => progress rewrite <-pred_Sn in *
+           | H : page_table_wf _ _ _ 0 |- _ => invert H
+           | H : page_table_wf _ _ _ ?lvl
+             |- page_table_wf _ _ _ (Nat.pred ?lvl) => invert H
+           | H : (forall level, _ -> get_index _ level _ < _)
+             |- context [get_index _ ?lvl _] => specialize (H lvl ltac:(solver))
+           | H : Forall ?P ?ls, H' : In ?x ?ls |- _ =>
+             rewrite Forall_forall in H; pose proof H; specialize (H _ H')
+           | H : nth_error _ _ = None |- _ => apply nth_error_None in H
+           | H : nth_error _ _ = Some _ |- _ => apply nth_error_In in H
+           | _ => apply IHlevel
+           | H : page_table_wf _ _ _ _ |- _ =>
+             invert H; basics; cbn [Datatypes.entries] in *; solver
+           | _ => break_match
+           | _ => solver
+           end.
+Qed.
+
+Lemma page_lookup_ok deref root_ptable s a :
+  address_wf a s ->
+  root_ptable_wf deref s root_ptable ->
+  page_lookup deref root_ptable s a <> None.
+Proof.
+  cbv [page_lookup root_ptable_wf address_wf]; basics.
+  match goal with
+  | H : ?i < ?l, H' : length ?ls = ?l |- context [nth_error ?ls ?i] =>
+    pose proof H; rewrite <-H', <-nth_error_Some in H
+  end.
+  break_match; [|solver].
+  match goal with
+  | H : Forall _ ?ls, H' : nth_error ?ls ?i = Some _ |- _ =>
+    rewrite Forall_forall in H;
+      specialize (H _ (nth_error_In _ _ H'))
+  end.
+  rewrite Nat.add_1_r.
+  apply page_lookup'_ok;
+    cbv [address_wf]; basics; try solver.
+Qed.
